@prefix rtc: <https://w3id.org/rtc#> .
@prefix xsd: <http://www.w3.org/2001/XMLSchema#> .
@prefix rdf: <http://www.w3.org/1999/02/22-rdf-syntax-ns#> .
@prefix rdfs: <http://www.w3.org/2000/01/rdf-schema#> .
@prefix owl: <http://www.w3.org/2002/07/owl#> .

rtc:Compound a rdfs:Class
        ; rdfs:label "Compound"
        ; rdfs:comment "A compound is a set of triples as an RDF resource."
.

rtc:elementOf a rdf:Property
        ; rdfs:label "element of"
        ; rdfs:comment "Assigns a triple to a compound as an element. The subject must be a RDF triple."
        ; rdfs:range rtc:Compound
        ; owl:inverseOf rtc:elements
.

rtc:elements a rdf:Property
        ; rdfs:label "elements"
        ; rdfs:comment "The set of all triples of a compound. The objects must be RDF triples."
        ; rdfs:domain rtc:Compound
        ; owl:inverseOf rtc:elementOf
.

rtc:subCompoundOf a rdf:Property
        ; rdfs:label "sub-compounds of"
        ; rdfs:comment "The subject compound is a sub-compound of the object compound, i.e. all triples of the sub-compound are elements of the super-compound."
        ; rdfs:domain rtc:Compound
        ; rdfs:range  rtc:Compound
.